tests/elab/vcgenImp.lean
@@ -149,8 +149,8 @@ theorem wpCmd_mono {Φ : Env} {c : Cmd} {Q Q' : State → Prop} (hQ : ∀ s, Q s
 abbrev Assn := Env → State → Prop
 
 instance : WP Cmd Unit Assn EStack⟨⟩ where
-  wpTrans c := ⟨fun Q _epost Φ s => wpCmd Φ c (Q () Φ) s⟩
-  wp_trans_monotone c := by
+  trans c := ⟨fun Q _epost Φ s => wpCmd Φ c (Q () Φ) s⟩
+  trans_monotone c := by
     intro Q Q' e e' _he hQ Φ s h
     exact wpCmd_mono (fun s' h' => hQ () Φ s' h') s h
 
